update

06_Examples.thy
@@ -5,47 +5,75 @@ theory "06_Examples"
 begin
 (*>*)
 
-chapter \<open>The Running Example\<close>
+chapter \<open>The Running Example in Isabelle\<close>
+
+text\<open>
+This chapter illustrates how the running example is implemented in Isabelle and highlights
+the corresponding correctness theorems for functions @{term \<E>arley_list}, @{term build_tree}, and
+@{term build_trees}. But first we make a small addition to easily compute if a grammar allows empty
+derivations or @{term "\<G> \<turnstile> [N] \<Rightarrow>\<^sup>* []"} holds for any non-terminal $N$ of grammar @{term \<G>}. We call
+a grammar @{term "\<epsilon>_free"} if there does not exists any production rule of the form $N \rightarrow \, \epsilon$.
+For a well-formed grammar, strictly speaking we only require the left-hand side of any production rule
+to be a non-terminal, we then prove a lemma stating that a grammar does only allow non-empty derivations
+for any non-terminal if and only if it is epsilon-free.
+\<close>
 
 definition \<epsilon>_free :: "'a cfg \<Rightarrow> bool" where
-  "\<epsilon>_free \<G> \<longleftrightarrow> (\<forall>r \<in> set (\<RR> \<G>). rule_body r \<noteq> [])"
+  "\<epsilon>_free \<G> \<equiv> \<forall>r \<in> set (\<RR> \<G>). rule_body r \<noteq> []"
 
-lemma \<epsilon>_free_impl_non_empty_deriv:
-  assumes "\<epsilon>_free \<G>"
-  shows "\<forall>N \<in> set (\<NN> \<G>). \<not> (\<G> \<turnstile> [N] \<Rightarrow>\<^sup>* [])"
+lemma nonempty_derives_iff_\<epsilon>_free:
+  assumes "wf_\<G> \<G>"
+  shows "nonempty_derives \<G> \<longleftrightarrow> \<epsilon>_free \<G>"
+(*<*)
+  sorry  
+(*>*)
+
+text\<open>
+Next we define the grammar $S ::= S + S \, | \, x$ in Isabelle. We introduce data types @{term T}, @{term N}, and @{term symbol}
+respectively representing terminal symbols $\{x, +\}$, the non-terminal $S$, and the type for symbols.
+Subsequently, we define the grammar as its four constituents: a list of non-terminal symbols, a list of terminal symbols,
+the production rules, and the start symbol. Finally, we specify the input $\omega = x + x + x$.
+\<close>
+
+datatype T = x | plus
+datatype N = S
+datatype symbol = Terminal T | Nonterminal N
+
+definition nonterminals :: "symbol list" where
+  "nonterminals = [Nonterminal S]"
+
+definition terminals :: "symbol list" where
+  "terminals = [Terminal x, Terminal plus]"
+
+definition rules :: "symbol rule list" where
+  "rules = [
+    (Nonterminal S, [Terminal x]),
+    (Nonterminal S, [Nonterminal S, Terminal plus, Nonterminal S])]"
+
+definition start_symbol :: symbol where
+  "start_symbol = Nonterminal S"
+
+definition \<G> :: "symbol cfg" where
+  "\<G> = CFG nonterminals terminals rules start_symbol"
+
+definition \<omega> :: "symbol list" where
+  "\<omega> = [Terminal x, Terminal plus, Terminal x, Terminal plus, Terminal x]"
+
+text\<open>
+The following three lemmas state the well-formedness of the grammar and input. The proofs are automatic
+by definition with addition of lemma @{thm[source] nonempty_derives_iff_\<epsilon>_free}.
+\<close>
+
+lemma wf_\<G>:
+  shows "wf_\<G> \<G>"
 (*<*)
   sorry  
 (*>*)
 
 text\<open>\<close>
 
-datatype t = x | plus
-datatype n = S
-datatype s = Terminal t | Nonterminal n
-
-definition nonterminals :: "s list" where
-  "nonterminals = [Nonterminal S]"
-
-definition terminals :: "s list" where
-  "terminals = [Terminal x, Terminal plus]"
-
-definition rules :: "s rule list" where
-  "rules = [
-    (Nonterminal S, [Terminal x]),
-    (Nonterminal S, [Nonterminal S, Terminal plus, Nonterminal S])
-  ]"
-
-definition start_symbol :: s where
-  "start_symbol = Nonterminal S"
-
-definition \<G> :: "s cfg" where
-  "\<G> = CFG nonterminals terminals rules start_symbol"
-
-definition \<omega> :: "s list" where
-  "\<omega> = [Terminal x, Terminal plus, Terminal x, Terminal plus, Terminal x]"
-
-lemma wf_\<G>:
-  shows "wf_\<G> \<G>"
+lemma nonempty_derives_\<G>:
+  shows "nonempty_derives \<G>"
 (*<*)
   sorry  
 (*>*)
@@ -58,18 +86,52 @@ lemma is_sentence_\<omega>:
   sorry  
 (*>*)
 
-text\<open>\<close>
+text\<open>
+This section concludes by illustrating the following main theorems for functions @{term "mbox0 (\<E>arley_list)"}, @{term build_tree}, and
+@{term build_trees} for the well-formed grammar @{term \<G>} and input @{term \<omega>} introduced above.
+\<close>
 
-lemma nonempty_derives:
-  shows "nonempty_derives \<G>"
+lemma correctness_bins:
+  shows "recognizing (bins (\<E>arley_list \<G> \<omega>)) \<G> \<omega> \<longleftrightarrow> \<G> \<turnstile> [\<SS> \<G>] \<Rightarrow>\<^sup>* \<omega>"
 (*<*)
   sorry  
 (*>*)
 
 text\<open>\<close>
 
-lemma correctness:
-  shows "recognizing (bins (\<E>arley_list \<G> \<omega>)) \<G> \<omega> \<longleftrightarrow> \<G> \<turnstile> [\<SS> \<G>] \<Rightarrow>\<^sup>* \<omega>"
+lemma wf_tree:
+  assumes "build_tree \<G> \<omega> (\<E>arley_list \<G> \<omega>) = Some t"
+  shows "wf_rule_tree \<G> t \<and> root_tree t = \<SS> \<G> \<and> yield_tree t = \<omega>"
+(*<*)
+  sorry  
+(*>*)
+
+text\<open>\<close>
+
+lemma correctness_tree:
+  shows "(\<exists>t. build_tree \<G> \<omega> (\<E>arley_list \<G> \<omega>) = Some t) \<longleftrightarrow> \<G> \<turnstile> [\<SS> \<G>] \<Rightarrow>\<^sup>* \<omega>"
+(*<*)
+  sorry  
+(*>*)
+
+text\<open>\<close>
+
+lemma wf_trees:
+  assumes "build_trees \<G> \<omega> (\<E>arley_list \<G> \<omega>) = Some fs"
+  assumes "f \<in> set fs"
+  assumes "t \<in> set (trees f)"
+  shows "wf_rule_tree \<G> t \<and> root_tree t = \<SS> \<G> \<and> yield_tree t = \<omega>"
+(*<*)
+  sorry  
+(*>*)
+
+text\<open>\<close>
+
+lemma soundness_trees:
+  assumes "build_trees \<G> \<omega> (\<E>arley_list \<G> \<omega>) = Some fs"
+  assumes "f \<in> set fs"
+  assumes "t \<in> set (trees f)"
+  shows "\<G> \<turnstile> [\<SS> \<G>] \<Rightarrow>\<^sup>* \<omega>"
 (*<*)
   sorry  
 (*>*)
