01_Introduction.thy
@@ -7,8 +7,9 @@ begin
 
 chapter\<open>Introduction\<close>
 
-text\<open>some introduction about parsing, formal development of correct algorithms: an example based on
-earley's recogniser, the benefits of formal methods, LocalLexing and the Bachelor thesis.\<close>
+text\<open>
+TODO
+\<close>
 
 section\<open>Related Work\<close>
 
@@ -47,66 +48,14 @@ They proof soundness and completeness for all non-left-recursive grammars using 
 
 section\<open>Structure\<close>
 
+text\<open>
+TODO
+\<close>
+
 section\<open>Contributions\<close>
 
 text\<open>
-SNIPPET:
-
-Context-free grammars have been used extensively for describing the syntax of programming languages
-and natural languages. Parsing algorithms for context-free grammars consequently play a large role in
-the implementation of compilers and interpreters for programming languages and of programs which understand
-or translate natural languages. Numerous parsing algorithms have been developed. Some are general,
-in the sense that they can handle all context-free grammars, while others can handle only subclasses of
-grammars. The latter, restricted algorithms tend to be much more efficient The algorithm described here
-seems to be the most efficient of the general algorithms, and also it can handle a larger class of grammars
-in linear time than most of the restricted algorithms.
-\<close>
-
-text\<open>
-SNIPPET:
-
-The Computer Science community has been able to automatically generate parsers for a very wide class of context
-free languages. However, many parsers are still written manually, either using tool support or even completely
-by hand. This is partly because in some application areas such as natural language processing and bioinformatics
-we don not have the luxury of designing the language so that it is amendable to know parsing techniques, but also
-it is clear that left to themselves computer language designers do not naturally write LR(1) grammars. A grammar
-not only defines the syntax of a language, it is also the starting point for the definition of the semantics,
-and the grammar which facilitates semantics definition is not usually the one which is LR(1). Given this difficulty
-in constructing natural LR(1) grammars that support desired semantics, the general parsing techniques, such as
-the CYK Younger \cite{Younger:1967}, Earley \cite{Earley:1970} and GLR Tomita \cite{Tomita:1985} algorithms, developed
-for natural language processing are also of interest to the wider computer science community. When using grammars as
-the starting point for semantics definition, we distinguish between recognizers which simply determine whether or not
-a given string is in the language defined by a given grammar, and parserwhich also return some form of derivation
-of the string, if one exists. In their basic form the CYK and Earley algorithms are recognizers while GLR-style
-algorithms are designed with derivation tree construction, and hence parsing, in mind.
-
-There is no known liner time parsing or recognition algorithm that can be used with all context free grammars.
-In their recognizer forms the CYK algorithm is worst case cubic on grammars in Chomsky normal form and Earley's
-algorithm is worst case cubic on general context free grammers and worst case n2 on non-ambibuous grammars.
-General recognizers must, by definition, be applicable to ambiguous grammars. Tomita's GLR algorithm is of unbounded
-polynomial order in the worst case. Expanding general recognizers to parser raises several problems, not least
-because there can be exponentially many or even infinitely many derivations for a given input string. A cubic
-recognizer which was modified to simply return all derivations could become an unbounded parser.
-Of course, it can be argued that ambiguous grammars reflect ambiguous semantics and thus should not be used in
-practice. This would be far too extreme a position to take. For example, it is well known that the if-else
-statement in hthe AnSI-standard grammar for C is ambiguous, but a longest match resolution results in a linear
-time parser that attach the else to the most recent if, as specified by the ANSI-C semantics. The ambiguous
-ANSI-C grammar is certainly practical for parser implementation. However, in general ambiguity is not so easily handled,
-and it is well known that grammar ambiguity is in fact undecidable Hopcroft \textit{et al} \cite{Hopcroft:2006}, thus
-we cannot expect a parser generator simply to check for ambiguity inthe grammar and report the problem back to the user.
-Another possiblity is to avoid the issue by just returning one derivation. However, if only one derivation is returned
-then this creates problems for a user who wants all derivations and, even in the case where only one derivation is
-required, there is the issue of ensuring that it is the required derivationthat is returned. A truely general parser
-will reutrn all possible derivations in some form. Perhaps the most well known representation is the shared packed
-parse foreset SPPF described and used by Tomita \cite{Tomita:1985}. Tomita's description of the representation does ont allow
-for the infinitely many derivations which arise from grammars which contain cycles, the source adapt the SPPF representation
-to allow these. Johnson \cite{Johnson:1991} has shown that Tomita-style SPPFs are worst case unbounded polynomial size. Thus
-using such structures will alo turn any cubic recognition technique into a worst case unbounded polynomial parsing technique.
-Leaving aside the potential increase in complexity when turning a recogniser into a parser, it is clear that this proccess is often difficult to carry
-out correctly. Earley gave an algorithm for constructing derivations of a string accepted by his recognizer,
-but this was subsequently shown by Tomita \cite{Tomita:1985} to return spurious derivations in certain cases.
-Tomita's original version of his algorithm failed to terminate on grammars with hidden left recursio and, as remarked above
-, had no mechanism for contructing complete SPPFs for grammers with cycles.
+TODO
 \<close>
 
 (*<*)
